thy/Simple_Firewall/SimpleFw_Semantics.thy
@@ -217,12 +217,18 @@ value[code] "simple_fw [
 subsection{*Reality check*}
 text{* While it is possible to construct a @{text "simple_fw"} expression that only matches a source
 or destination port, such a match is not meaningful, as the presence of the port information is 
-dependent on the protocol. Thus, a match for a port should always include the match for a protocol.*}
+dependent on the protocol. Thus, a match for a port should always include the match for a protocol.
+Additionally, prefixes should be zero on bits beyond the prefix length.
+*}
+
+definition "valid_prefix_fw m = valid_prefix (split PrefixMatch m)"
 
 definition "simple_match_valid m \<equiv> 
-(({p. simple_match_port (sports m) p} \<noteq> UNIV (*\<and> {p. simple_match_port (sports m) p} \<noteq> {}*)) \<or> 
+(((({p. simple_match_port (sports m) p} \<noteq> UNIV (*\<and> {p. simple_match_port (sports m) p} \<noteq> {}*)) \<or> 
 ({p. simple_match_port (dports m) p} \<noteq> UNIV (*\<and> {p. simple_match_port (dports m) p} \<noteq> {}*))) 
-\<longrightarrow> (proto m \<in> Proto `{TCP, UDP, SCTP})" 
+\<longrightarrow> (proto m \<in> Proto `{TCP, UDP, SCTP})) \<and>
+valid_prefix_fw (src m) \<and> valid_prefix_fw (dst m)
+)" 
 
 lemma simple_match_valid_alt_hlp1: "{p. simple_match_port x p} \<noteq> UNIV \<longleftrightarrow> (case x of (s,e) \<Rightarrow> s \<noteq> 0 \<or> e \<noteq> max_word)"
 	apply(clarsimp simp: set_eq_UNIV split: prod.splits)
@@ -233,7 +239,8 @@ done
 lemma simple_match_valid_alt_hlp2: "{p. simple_match_port x p} \<noteq> {} \<longleftrightarrow> (case x of (s,e) \<Rightarrow> s \<le> e)" by auto
 lemma simple_match_valid_alt[code_unfold]: "simple_match_valid = (\<lambda> m.
 	(let c = (\<lambda>(s,e). (*s \<le> e \<and>*) (s \<noteq> 0 \<or> e \<noteq> max_word)) in (
-	if c (sports m) \<or> c (dports m) then proto m = Proto TCP \<or> proto m = Proto UDP \<or> proto m = Proto SCTP else True)))
+	if c (sports m) \<or> c (dports m) then proto m = Proto TCP \<or> proto m = Proto UDP \<or> proto m = Proto SCTP else True)) \<and>
+valid_prefix_fw (src m) \<and> valid_prefix_fw (dst m))
 " 
 unfolding fun_eq_iff
 unfolding simple_match_valid_def Let_def
